ConstrainedDecodingFormalization/Lexing.lean
@@ -91,6 +91,20 @@ def LexerSpec.seq_term (spec: LexerSpec α Γ σ) (seq: List α) : Option Γ :=
   | some s => spec.term s
   | none => none
 
+def LexerSpec.accept_seq_term (spec: LexerSpec α Γ σ) (seq: List α) (h: seq ∈ spec.automaton.accepts) : Γ :=
+  let s := (spec.automaton.eval seq).get <| by
+    simp[FSA.accepts, FSA.acceptsFrom] at h
+    rw[Set.mem_setOf] at h
+    have ⟨e, he⟩ := h
+    simp[FSA.eval, he]
+  have sa : s ∈ spec.automaton.accept := by
+    simp[FSA.accepts, FSA.acceptsFrom] at h
+    rw[Set.mem_setOf] at h
+    have ⟨e, he⟩ := h
+    simp[s, he]
+  let term := spec.term s
+  term.get ((spec.hterm s).mp sa)
+
 def Lexer (α : Type u) (Γ : Type v) := List (Ch α) -> Option (List (Ch Γ) × List α)
 
 inductive PartialLexRel (spec: LexerSpec α Γ σ)
@@ -99,14 +113,20 @@ inductive PartialLexRel (spec: LexerSpec α Γ σ)
 | nil :
     PartialLexRel spec
       [] [] []
+-- case 0 (unmentioned in paper but implicitly done in the lexing transducer)
+| step_nil_eos { w wn tokens }:
+    PartialLexRel spec w tokens [] →
+    wn = w ++ [ExtChar.eos] →
+    [] ∉ spec.automaton.accepts →
+    PartialLexRel spec wn (tokens ++ [.eos]) []
   -- case 1
 | step_eos {w wn tokens unlexed} :
     PartialLexRel spec w tokens unlexed →
     -- this nonsense needs to be done to satisfy the eliminator for some reason
     -- related? https://github.com/leanprover/lean4/issues/9803
     wn = w ++ [ExtChar.eos] →
-    unlexed ∈ spec.automaton.accepts →
-      PartialLexRel spec wn (tokens ++ [.eos]) []
+    (h : unlexed ∈ spec.automaton.accepts) →
+      PartialLexRel spec wn (tokens ++ [.char (spec.accept_seq_term unlexed h), .eos]) []
   -- case 2
 | step_char_continue {w wn tokens unlexed ch} :
     PartialLexRel spec w tokens unlexed →
@@ -114,13 +134,14 @@ inductive PartialLexRel (spec: LexerSpec α Γ σ)
     unlexed ++ [ch] ∈ spec.automaton.prefixLanguage →
       PartialLexRel spec wn tokens (unlexed ++ [ch])
   -- case 3
-| step_char_commit {w wn tokens unlexed ch t} :
+| step_char_commit {w wn tokens unlexed ch} :
     PartialLexRel spec w tokens unlexed →
     wn = w ++ [ExtChar.char ch] →
-    -- next is not in prefix language, but current is in accept
+    -- next is not in prefix language, but current is in accept, and ch is a prefix of something
     unlexed ++ [ch] ∉ spec.automaton.prefixLanguage →
-    some t = spec.seq_term unlexed →
-      PartialLexRel spec wn (tokens ++ [ExtChar.char t]) [ch]
+    [ch] ∈ spec.automaton.prefixLanguage →
+    (h : unlexed ∈ spec.automaton.accepts) →
+      PartialLexRel spec wn (tokens ++ [ExtChar.char (spec.accept_seq_term unlexed h)]) [ch]
 
 private def PartialLex_trans (spec: LexerSpec α Γ σ) (prev: Option (List (Ch Γ) × List α))
    (c : Ch α) : Option (List (Ch Γ) × List α) :=
@@ -129,14 +150,16 @@ private def PartialLex_trans (spec: LexerSpec α Γ σ) (prev: Option (List (Ch 
   | some (tokens, unlexed) =>
     match c with
     | ExtChar.eos =>
-      if unlexed ∈ spec.automaton.accepts then
+      if h : unlexed ∈ spec.automaton.accepts then
+        some (tokens ++ [.char (spec.accept_seq_term unlexed h), .eos], [])
+      else if unlexed = [] then
         some (tokens ++ [.eos], [])
       else
         none
     | ExtChar.char ch =>
       let new_unlexed := unlexed ++ [ch]
       match spec.automaton.eval new_unlexed with
-      | some σ' => some (tokens, new_unlexed)
+      | some _ => some (tokens, new_unlexed)
       | none =>
         let dst := spec.automaton.eval unlexed
         match dst with
@@ -145,19 +168,82 @@ private def PartialLex_trans (spec: LexerSpec α Γ σ) (prev: Option (List (Ch 
           if h : σ ∈ spec.automaton.accept then
             let term := spec.term σ
             have h2 := (spec.hterm σ).mp h
-            match hc : term with
-            | some t => some (tokens ++ [ExtChar.char t], [ch])
-            | none => by
-              simp[term] at hc
-              simp_all
+            let t := term.get h2
+            if (spec.automaton.eval [ch]).isSome then
+              some (tokens ++ [ExtChar.char t], [ch])
+            else
+              none
           else
             none
 
+@[simp]
+private def PartialLex_trans_nil (spec: LexerSpec α Γ σ) (c : Ch α) :
+  PartialLex_trans spec none c = none := by
+  simp[PartialLex_trans]
+
+@[simp]
+private def PartialLex_trans_foldl_nil (spec: LexerSpec α Γ σ) (ws : List (Ch α)) :
+  foldl (PartialLex_trans spec) none ws = none := by
+  exact foldl_fixed' (congrFun rfl) ws
+
+@[simp]
 private def PartialLex_seed (spec: LexerSpec α Γ σ) (seed: Option (List (Ch Γ) × List α)) : Lexer α Γ :=
   fun w => List.foldl (PartialLex_trans spec) seed w
 
+@[simp]
 def PartialLex (spec: LexerSpec α Γ σ) : Lexer α Γ :=
   PartialLex_seed spec (some ([], []))
+
+
+inductive LexingState (σ : Type w) where
+| id : σ → LexingState σ
+| start : LexingState σ
+deriving DecidableEq, Repr
+
+def LexingState.src {σ : Type w} (spec: LexerSpec α Γ σ) : LexingState σ → σ
+| LexingState.id s => s
+| LexingState.start => spec.automaton.start
+
+@[simp]
+lemma LexingState_src_id {σ : Type w} (spec: LexerSpec α Γ σ) (s : σ) :
+  LexingState.src spec (LexingState.id s) = s := by
+  simp[LexingState.src]
+
+/-- Given a lexing automaton `A`, build a character-to-token lexing FST with output over `Γ`
+    For the lexing FSA, we'll use the convention that each terminal symbol is attached to an accept state (see Fig. 1) -/
+def BuildLexingFST (spec: LexerSpec α Γ σ) :
+    FST (Ch α) (Ch Γ) (LexingState σ) := Id.run do
+  let ⟨A, term, hterm, _⟩ := spec
+
+  let new_q0 := LexingState.start
+  let q0 := spec.automaton.start
+  let F := A.accept
+
+  let step := fun (q : LexingState σ) (c : Ch α) =>
+    let qorg := LexingState.src spec q
+    match c with
+    | ExtChar.char c =>
+      if h : (A.step qorg c).isSome then
+        some (LexingState.id ((A.step qorg c).get h), [])
+      else if h : qorg ∈ F then
+        let T := (term qorg).get <| ((hterm qorg).mp h)
+        A.step q0 c |>.map (fun q' => (LexingState.id q', [ExtChar.char T]))
+      else
+        none
+    | ExtChar.eos =>
+      if h : qorg ∈ F then
+        let T := (term qorg).get <| (hterm qorg).mp h
+        some (new_q0, [T, .eos])
+      else if q = new_q0 then
+        some (new_q0, [.eos])
+      else
+        none
+
+  ⟨new_q0, step, [new_q0]⟩
+
+@[simp]
+def LexingFST_start (spec: LexerSpec α Γ σ) : (BuildLexingFST spec).start = LexingState.start := by
+  simp[BuildLexingFST, Id.run]
 
 lemma PartialLex_pruned_eq_PartialLexRel_seed (spec: LexerSpec α Γ σ) (hp: spec.automaton.pruned) :
     (∀ w tokens unlexed, (PartialLexRel spec w tokens unlexed) → PartialLex_seed spec (some ([], [])) w = some (tokens, unlexed)) ∧
@@ -169,10 +255,14 @@ lemma PartialLex_pruned_eq_PartialLexRel_seed (spec: LexerSpec α Γ σ) (hp: sp
     induction h
     case nil =>
       simp[PartialLex, PartialLex_seed, PartialLex_trans]
-    case step_eos w wn tokens unlexed ih wwn h hacc =>
+    case step_nil_eos w wn tokens ih wwn h hacc =>
       simp[PartialLex, PartialLex_seed, PartialLex_trans] at hacc ⊢
       simp[wwn, hacc, PartialLex_trans]
       exact h
+    case step_eos w wn tokens unlexed ih wwn h hacc =>
+      simp[PartialLex, PartialLex_seed, PartialLex_trans] at hacc ⊢
+      simp[wwn, hacc, PartialLex_trans]
+      simp[h]
     case step_char_continue w wn tokens unlexed ch ih wwn h hacc =>
       simp[PartialLex, PartialLex_seed, PartialLex_trans] at hacc ⊢
       simp[wwn, hacc, PartialLex_trans]
@@ -184,25 +274,32 @@ lemma PartialLex_pruned_eq_PartialLexRel_seed (spec: LexerSpec α Γ σ) (hp: sp
       | some σ' =>
         simp at he
         simp[he]
-    case step_char_commit w wn tokens unlexed ch t ih wwn hni ht hacc =>
+    case step_char_commit w wn tokens unlexed ch ih wwn hni hc_pfx ht hacc =>
       simp[PartialLex, PartialLex_seed, PartialLex_trans] at hacc ⊢
       simp[wwn, hacc, PartialLex_trans]
       cases he: spec.automaton.eval (unlexed ++ [ch]) with
       | none =>
         simp[FSA.eval] at he
         simp[he]
-        simp[LexerSpec.seq_term] at ht
-        split at ht
-        case h_1 st heq =>
-          simp[heq]
-          have : st ∈ spec.automaton.accept := by
-            apply (spec.hterm st).mpr
-            simp[←ht]
-          exists this
-          split
-          <;> simp_all
-        case h_2 heq =>
-          simp[heq] at ht
+        simp[LexerSpec.accept_seq_term, FSA.accepts, FSA.acceptsFrom] at ht
+        split
+        <;> simp_all
+        rw[Set.mem_setOf] at ht
+        have ⟨e, he'⟩ := ht
+        rename_i σ' _ heq
+        simp[he'] at heq
+        constructor
+        rw[←hprune] at hc_pfx
+        simp[FSA.intermediateLanguage] at hc_pfx
+        rw[Set.mem_setOf] at hc_pfx ht
+        cases hch : spec.automaton.evalFrom spec.automaton.start [ch]
+        <;> simp_all
+        rename_i heq'
+        rw[Set.mem_setOf] at ht
+        simp[heq'] at ht
+        exists ht
+        rename_i ht' _ _
+        simp[heq', LexerSpec.accept_seq_term, FSA.accepts, FSA.acceptsFrom]
       | some σ' =>
         have : spec.automaton.evalFrom spec.automaton.start (unlexed ++ [ch]) = none := by
           simp[←hprune] at hni
@@ -221,6 +318,10 @@ lemma PartialLex_pruned_eq_PartialLexRel_seed (spec: LexerSpec α Γ σ) (hp: sp
       simp[PartialLex_seed] at h
       cases h.left
       <;> simp_all
+      case step_nil_eos =>
+        have ⟨hl, htokens, _⟩ := h
+        simp[←htokens]
+        exact hl
       case step_eos =>
         have ⟨hl, htokens, _⟩ := h
         simp[←htokens]
@@ -234,7 +335,7 @@ lemma PartialLex_pruned_eq_PartialLexRel_seed (spec: LexerSpec α Γ σ) (hp: sp
         simp[←htokens, ←hunlexed]
         exact hl
     case cons ch tail ih =>
-      have my_inductive_seed:= h.left
+      have my_inductive_seed := h.left
       have computable_eq_some := left wp seed_f seed_s my_inductive_seed
       have h_token_unlexed := h.right
 
@@ -254,22 +355,41 @@ lemma PartialLex_pruned_eq_PartialLexRel_seed (spec: LexerSpec α Γ σ) (hp: sp
         match ch with
         | ExtChar.eos =>
           simp[PartialLex_trans] at hns
-
-          have haccept : seed_s ∈ spec.automaton.accepts := by exact hns.left
-          let new_tokens := seed_f ++ [.eos]
-          have step := PartialLexRel.step_eos my_inductive_seed rfl haccept
-          have ihr := ih (wp ++ [ExtChar.eos]) new_tokens []
-          have ihr := by
-            apply ihr
-            constructor
-            exact step
-            simp[PartialLex_seed]
-            simp[←hns.right.left, ←hns.right.right, new_tokens] at h_token_unlexed ⊢
-            exact h_token_unlexed
-          suffices wp ++ ExtChar.eos :: tail = (wp ++ [ExtChar.eos]) ++ tail by
-            rw[this]
-            exact ihr
-          exact append_cons wp ExtChar.eos tail
+          by_cases haccept : seed_s ∈ spec.automaton.accepts
+          . let new_tokens := seed_f ++ [.char (spec.accept_seq_term seed_s haccept), .eos]
+            have step := PartialLexRel.step_eos my_inductive_seed rfl haccept
+            have ihr := ih (wp ++ [ExtChar.eos]) new_tokens []
+            have ihr := by
+              apply ihr
+              constructor
+              exact step
+              simp[PartialLex_seed]
+              simp[haccept] at hns
+              have := h_token_unlexed
+              simp[←hns.left, ←hns.right, new_tokens] at h_token_unlexed ⊢
+              exact h_token_unlexed
+            suffices wp ++ ExtChar.eos :: tail = (wp ++ [ExtChar.eos]) ++ tail by
+              rw[this]
+              exact ihr
+            exact append_cons wp ExtChar.eos tail
+          . simp[haccept] at hns
+            let new_tokens := seed_f ++ [.eos]
+            simp[hns.left] at my_inductive_seed
+            simp[hns] at haccept
+            have step := PartialLexRel.step_nil_eos my_inductive_seed rfl haccept
+            have ihr := ih (wp ++ [ExtChar.eos]) new_tokens []
+            have ihr := by
+              apply ihr
+              constructor
+              exact step
+              simp[PartialLex_seed]
+              have := h_token_unlexed
+              simp[←hns.right, new_tokens] at h_token_unlexed ⊢
+              exact h_token_unlexed
+            suffices wp ++ ExtChar.eos :: tail = (wp ++ [ExtChar.eos]) ++ tail by
+              rw[this]
+              exact ihr
+            exact append_cons wp ExtChar.eos tail
         | ExtChar.char ch =>
           simp[PartialLex_trans] at hns
           cases hp : spec.automaton.evalFrom spec.automaton.start (seed_s ++ [ch]) with
@@ -301,62 +421,70 @@ lemma PartialLex_pruned_eq_PartialLexRel_seed (spec: LexerSpec α Γ σ) (hp: sp
             cases ha : spec.automaton.evalFrom spec.automaton.start seed_s with
             | none => simp[hp, ha] at hns
             | some σ =>
-              simp[hp, ha] at hns
+              simp_all[hp, ha]
+              cases hbo : spec.automaton.eval [ch]
+              . simp at hbo
+                simp[hbo] at hns
+              . have hint : (seed_s ++ [ch] ∉ spec.automaton.intermediateLanguage) := by
+                  simp [FSA.intermediateLanguage]
+                  rw[Set.mem_setOf]
+                  simp[←hns.right.right] at hp
+                  simp [hp]
+                have hpfx : (seed_s ++ [ch] ∉ spec.automaton.prefixLanguage) := by
+                  rw[←hprune]
+                  exact hint
 
-              have hint : (seed_s ++ [ch] ∉ spec.automaton.intermediateLanguage) := by
-                simp [FSA.intermediateLanguage]
-                rw[Set.mem_setOf]
-                simp [hp]
-              have hpfx : (seed_s ++ [ch] ∉ spec.automaton.prefixLanguage) := by
-                rw[←hprune]
-                exact hint
+                have haccept : (seed_s ∈ spec.automaton.accepts) := by
+                  have ⟨⟨h, _⟩, ht⟩ := hns.right
+                  simp[FSA.accepts, FSA.acceptsFrom]
+                  rw[Set.mem_setOf]
+                  exists σ
 
-              have haccept : (seed_s ∈ spec.automaton.accepts) := by
-                have ⟨t, ht⟩ := hns
-                simp[FSA.accepts, FSA.acceptsFrom]
-                rw[Set.mem_setOf]
-                exists σ
+                -- very round about away but works
+                let term := spec.term σ
+                have ⟨t, ht⟩ : ∃ t, term = some t := by
+                  have ⟨⟨h, _⟩, ht⟩ := hns.right
+                  have h2 := (spec.hterm σ).mp h
+                  match hc: term with
+                  | none =>
+                    simp[term] at hc
+                    simp[hc] at h2
+                  | some t => exists t
 
-              -- quite round about away but works
-              let term := spec.term σ
-              have ⟨t, ht⟩ : ∃ t, term = some t := by
-                have ⟨ha, ht⟩ := hns
-                have h2 := (spec.hterm σ).mp ha
-                match hc: term with
-                | none =>
-                  simp[term] at hc
-                  simp[hc] at h2
-                | some t => exists t
+                let tused := spec.accept_seq_term seed_s haccept
+                have htused : t = tused := by
+                  simp[term] at ht
+                  simp[tused, LexerSpec.accept_seq_term]
+                  conv =>
+                    rhs
+                    pattern spec.automaton.evalFrom spec.automaton.start seed_s
+                    rw[ha]
+                  simp[ht]
+                let new_tokens := seed_f ++ [ExtChar.char tused]
+                let new_unlexed := [ch]
 
-              let new_tokens := seed_f ++ [ExtChar.char t]
-              let new_unlexed := [ch]
-
-              have ihr := ih (wp ++ [ExtChar.char ch]) new_tokens new_unlexed
-              have ihr := by
-                apply ihr
-                constructor
-                apply PartialLexRel.step_char_commit my_inductive_seed
-                simp[PartialLex_seed]
-                exact hpfx
-                simp[term] at ht
-                simp[LexerSpec.seq_term]
-                simp[ha, ht]
-                simp[PartialLex_seed, new_tokens, new_unlexed, hns]
-                have ⟨ha, ht'⟩ := hns
-                split at ht'
-                case h_1 heq =>
-                  have := h_token_unlexed
+                have ihr := ih (wp ++ [ExtChar.char ch]) new_tokens new_unlexed
+                have ihr : PartialLexRel spec (wp ++ [ExtChar.char ch] ++ tail) tokens unlexed := by
+                  have ⟨⟨_, hseed⟩, ht'⟩ := hns.right
+                  apply ihr
+                  apply PartialLexRel.step_char_commit h.left
+                  simp[PartialLex_seed]
+                  exact hpfx
+                  simp[PartialLex_seed, new_tokens, new_unlexed, hns]
                   simp_all
-                  simp[←ht'.left, ←ht'.right] at this ⊢
-                  simp[heq, ht, term] at ht
-                  rw[←ht]
-                  exact this
-                case h_2 heq =>
-                  simp[heq, ht, term] at ht
-              suffices wp ++ ExtChar.char ch :: tail = (wp ++ [ExtChar.char ch]) ++ tail by
-                rw[this]
-                exact ihr
-              exact append_cons wp (ExtChar.char ch) tail
+                  simp[term] at ht
+                  simp[ht] at hseed
+                  rw[←hprune]
+                  simp[FSA.intermediateLanguage]
+                  rw[Set.mem_setOf]
+                  rw[hbo]
+                  simp
+                  simp[new_tokens, new_unlexed, ←ht', ←hseed, ←htused, ht, term] at h_token_unlexed ⊢
+                  exact h_token_unlexed
+                suffices wp ++ ExtChar.char ch :: tail = (wp ++ [ExtChar.char ch]) ++ tail by
+                  rw[this]
+                  exact ihr
+                exact append_cons wp (ExtChar.char ch) tail
 
 theorem PartialLex_pruned_eq_PartialLexRel (spec: LexerSpec α Γ σ) (hp: spec.automaton.pruned) :
     ∀ w tokens unlexed, (PartialLexRel spec w tokens unlexed) ↔ PartialLex spec w = some (tokens, unlexed)
@@ -374,74 +502,417 @@ theorem PartialLex_pruned_eq_PartialLexRel (spec: LexerSpec α Γ σ) (hp: spec.
     simp at this
     exact this
 
-
-/-- Given a lexing automaton `A`, build a character-to-token lexing FST with output over `Γ`
-    For the lexing FSA, we'll use the convention that each terminal symbol is attached to an accept state (see Fig. 1) -/
-def BuildLexingFST (spec: LexerSpec α Γ σ) :
-    FST (Ch α) (Ch Γ) σ := Id.run do
-  let ⟨A, term, hterm, _⟩ := spec
-
-  let q0 := A.start
-  let F := A.accept
-
-  let step := fun (q : σ) (c : Ch α) =>
-    match c with
-    | ExtChar.char c =>
-      if h : (A.step q c).isSome then
-        some ((A.step q c).get h, [])
-      else if h : q ∈ F then
-        let T := (term q).get <| ((hterm q).mp h)
-        A.step q0 c |>.map (fun q' => (q', [ExtChar.char T]))
-      else
-        none
-    | ExtChar.eos =>
-      if h : q ∈ F then
-        let T := (term q).get <| ((hterm q).mp h)
-        some (q0, [T, .eos])
-      else if q = q0 then
-        some (q0, [.eos])
-      else
-        none
-
-  ⟨q0, step, [q0]⟩
-
-def LexingFST_trans_iff_PartialLex (spec: LexerSpec α Γ σ) (h: [] ∉ spec.automaton.accepts) :
-  ∀ w ts,
-      (∀ wr, PartialLex spec w = some (ts, wr) →
-        (∃ q', ((BuildLexingFST spec).eval w = some (q', ts)) ∧
-                (BuildLexingFST spec).eval wr = some (q', []))) ∧
-      (∀ q', (BuildLexingFST spec).eval w = some (q', ts) → ∃ wr, PartialLex spec w = some (ts, wr))
-            := by
-  intro w ts
-  -- evalFrom fold matches lex foldl more nicely induction wise
-  suffices ∀ seed, (∀ wr, PartialLex_seed spec seed w = some (ts, wr) →
-        (∃ q', ((BuildLexingFST spec).evalFrom_fold_seed w seed = some (q', ts)) ∧
-                (BuildLexingFST spec).evalFrom_fold wr = some (q', []))) ∧
-      (∀ q', (BuildLexingFST spec).eval_fold w = some (q', ts) → ∃ wr, PartialLex_seed spec seed w = some (ts, wr)) by
-    simp[FST.eval_fold_eq_eval] at this
-    exact this
-
-  induction w generalizing ts
+-- automata parsing iff LexingFst parses and does not produce tokens
+private def FSA_ch_to_LexingFST (spec: LexerSpec α Γ σ) :
+  ∀ (w : List α) q q', (q ≠ LexingState.start ∨ w ≠ []) →
+    (spec.automaton.evalFrom (q.src spec) w = some q' ↔
+    (BuildLexingFST spec).evalFrom q w = some (LexingState.id q', []))
+    := by
+  intro w q q' h
+  induction w generalizing q q'
   case nil =>
-    simp[FST.eval_fold, FST.evalFrom_fold, FST.evalFrom_fold_seed]
-    apply And.intro
-    . intro wr
-      intro h
-      simp[PartialLex] at h
-      constructor
-      exact h.left
-      simp[h.right]
-    . intro hl
-      simp[PartialLex]
-      exact hl
-  case cons head tail ih =>
-    constructor
-    . intro wr
-      intro h
-      simp[PartialLex] at h
-      rw[List.foldl.eq_def] at h
+    simp[LexingState.src]
+    simp at h
+    split
+    case h_1 x s => simp
+    case h_2 s => simp at h
+  case cons hd tl ih =>
+    simp[FSA.evalFrom]
+    simp[FST.eval, FST.evalFrom] at h
+    cases hstep : spec.automaton.step (LexingState.src spec q) hd
+    . simp[FST.evalFrom]
+      nth_rewrite 1 [BuildLexingFST, Id.run]
+      simp[hstep]
+      by_cases haccept: LexingState.src spec q ∈ spec.automaton.accept
+      simp_all
+      split <;> simp_all
+      split <;> simp_all
+      intro _ h
+      rename_i heq _ _ _ _ _
+      have ⟨e, hw⟩ := heq
+      simp[←hw.right] at h
+      simp[haccept]
+    . rename_i astep
+      have : (spec.automaton.step (LexingState.src spec q) hd).isSome := by
+        simp[hstep]
+      simp[FST.evalFrom]
+      conv =>
+        pattern (BuildLexingFST spec).step q
+        unfold BuildLexingFST
+      simp[Id.run, this]
+      simp[hstep]
+      have ih := ih (LexingState.id astep) q' (by simp)
+      simp[LexingState.src] at ih
+      convert ih
+      split <;> simp_all
 
-    . sorry
+private def PartialLex_to_LexingFST_evalFold (spec: LexerSpec α Γ σ) (he: [] ∉ spec.automaton.accepts) :
+  ∀ wp ws q' seed_ts seed_wr,
+       PartialLex spec wp = some (seed_ts, seed_wr) →
+      (BuildLexingFST spec).eval wp = some (q', seed_ts) →
+      (BuildLexingFST spec).eval seed_wr = some (q', []) →
+      (seed_wr = [] ↔ q' = LexingState.start) →
+      match PartialLex_seed spec (some (seed_ts, seed_wr)) ws with
+      | some (ts, wr) =>
+        (∃ q'', ((BuildLexingFST spec).evalFrom_fold_seed q' ws seed_ts = some (q'', ts)) ∧
+                 (BuildLexingFST spec).evalFrom_fold_seed (BuildLexingFST spec).start wr [] = some (q'', []))
+      | none => (BuildLexingFST spec).evalFrom_fold_seed q' ws seed_ts = none := by
+  intro wp ws q' seed_ts seed_wr
+  let fst := BuildLexingFST spec
+  let new_q0 := fst.start
+  let old_q0 := spec.automaton.start
+
+  have h_q0_na : old_q0 ∉ spec.automaton.accept := by
+    by_contra h'
+    simp[FSA.accepts_iff] at he
+    have : spec.automaton.evalFrom old_q0 [] = some old_q0 := by
+      simp[FSA.evalFrom_nil]
+    have w : ∃ f, spec.automaton.evalFrom spec.automaton.start [] = some f ∧ f ∈ spec.automaton.accept := by
+      exists old_q0
+    simp at w
+    exact he w
+
+  induction ws generalizing wp q' seed_ts seed_wr
+  <;> (
+    intro h₀ h₁ h₂ h₃
+    have h₂_fsa : spec.automaton.evalFrom spec.automaton.start seed_wr = some (LexingState.src spec q') := by
+      by_cases hempty : seed_wr = []
+      . simp[hempty, h₃]
+        have := h₃.mp hempty
+        simp[LexingState.src, this]
+      . have : q' ≠ LexingState.start := by
+          exact (Iff.ne h₃).mp hempty
+        have hbase := (FSA_ch_to_LexingFST spec (seed_wr) LexingState.start (q'.src spec) (Or.inr hempty)).mpr (by
+          convert h₂
+          cases q' <;> simp_all
+        )
+        simp[LexingState.src] at hbase ⊢
+        cases q' <;> simp_all
+
+    simp[FST.eval, FST.eval_fold, FST.evalFrom_fold, FST.evalFrom_fold_seed]
+    rw[←FST.eval_fold_eq_eval] at h₂
+    simp[FST.eval_fold, FST.evalFrom_fold] at h₂
+  )
+  case nil =>
+    exact h₂
+  case cons head tail ih =>
+    let pl_step := (PartialLex_trans spec (some (seed_ts, seed_wr)) head)
+    cases hh : head
+    case eos =>
+      simp[PartialLex_trans]
+      let afinal := spec.automaton.eval seed_wr
+      by_cases haccept : seed_wr ∈ spec.automaton.accepts
+      . simp[haccept]
+        have ⟨aq', haq'⟩ := spec.automaton.accepts_iff.mp haccept
+        have : spec.automaton.evalFrom (LexingState.src spec LexingState.start) seed_wr = some aq' := by
+          simp[LexingState.src, haq']
+        -- this shows that the state at the fst is "accepting" in the fsa
+        have hfsa := (FSA_ch_to_LexingFST spec (seed_wr) LexingState.start aq'
+           (by simp; by_contra ha; rw[ha] at haccept; contradiction)).mp this
+
+        have hq'aq' : q' = LexingState.id aq' := by
+          rw[FST.evalFrom_fold_seed_eq_evalFrom_seed] at h₂
+          simp[FST.evalFrom_seed] at h₂
+          simp at hfsa
+          simp[hfsa] at h₂
+          exact Eq.symm h₂
+
+        -- find out the token that is produced
+        let produced_token := spec.accept_seq_term seed_wr haccept
+        -- have hseq_term : aq = spec_term
+        have hlex_trans :
+          (BuildLexingFST spec).evalFrom_fold_step (some (q', seed_ts)) head = some (LexingState.start, seed_ts ++ [ExtChar.char produced_token, ExtChar.eos]) := by
+          simp at h₁ ⊢
+          rw[←FST.evalFrom_fold_eq_evalFrom] at h₁
+          simp[FST.evalFrom_fold_seed] at h₁ ⊢
+          simp[FST.evalFrom_fold_step, BuildLexingFST, Id.run, hh]
+          simp[hq'aq', LexingState.src, haq']
+          simp[produced_token]
+          simp[LexerSpec.accept_seq_term]
+          have : afinal = spec.automaton.evalFrom spec.automaton.start seed_wr := by simp[afinal]
+          conv =>
+            rhs
+            pattern spec.automaton.evalFrom spec.automaton.start seed_wr
+            rw[←this]
+          simp[haq', this]
+
+        have hlex_wp_step : (BuildLexingFST spec).eval (wp ++ [head]) = some (LexingState.start, seed_ts ++ [.char produced_token, ExtChar.eos]) := by
+          simp[FST.evalFrom, FST.eval] at h₁ ⊢
+          rw[←FST.evalFrom_fold_eq_evalFrom] at h₁ ⊢
+          simp[FST.evalFrom_fold, FST.evalFrom_fold_seed] at h₁ ⊢
+          rw[h₁]
+          exact hlex_trans
+
+        have hplex_step : PartialLex spec (wp ++ [head]) = some (seed_ts ++ [.char produced_token, ExtChar.eos], []) := by
+          simp[PartialLex, PartialLex_seed] at h₀ ⊢
+          rw[h₀]
+          simp[PartialLex_trans, hh]
+          simp[produced_token]
+          simp[haccept]
+
+        have lex_wr_step : (BuildLexingFST spec).eval [] = some (LexingState.start, []) := by
+          simp[BuildLexingFST, Id.run, FST.eval, FST.evalFrom]
+        have ih := ih (wp ++ [head]) LexingState.start (seed_ts ++ [.char produced_token, ExtChar.eos]) [] hplex_step hlex_wp_step lex_wr_step
+
+        simp[hh] at hlex_trans
+        rw[hlex_trans]
+        simp[produced_token] at ih
+
+        convert ih
+      . simp[haccept]
+        by_cases hempty : seed_wr = []
+        . simp at hempty
+          have hlex_trans :
+            (BuildLexingFST spec).evalFrom_fold_step (some (q', seed_ts)) head = some (LexingState.start, seed_ts ++ [ExtChar.eos]) := by
+            simp[FST.evalFrom, FST.eval] at h₁ ⊢
+            rw[←FST.evalFrom_fold_eq_evalFrom] at h₁
+            simp[FST.evalFrom_fold, FST.evalFrom_fold_seed] at h₁ ⊢
+            simp[FST.evalFrom_fold_step, BuildLexingFST, Id.run, hh]
+            -- what q' is when seed_wr = []
+            have hq'_start : q' = LexingState.start := by
+              rw[FST.evalFrom_fold_seed_eq_evalFrom_seed] at h₂
+              simp[FST.evalFrom_seed, hempty] at h₂
+              exact Eq.symm h₂
+            simp[hq'_start, LexingState.src]
+            simp[old_q0] at h_q0_na
+            simp[h_q0_na]
+
+          have hlex_wp_step : (BuildLexingFST spec).eval (wp ++ [head]) = some (LexingState.start, seed_ts ++ [ExtChar.eos]) := by
+            simp[FST.evalFrom, FST.eval] at h₁ ⊢
+            rw[←FST.evalFrom_fold_eq_evalFrom] at h₁ ⊢
+            simp[FST.evalFrom_fold, FST.evalFrom_fold_seed] at h₁ ⊢
+            rw[h₁]
+            exact hlex_trans
+
+          have hplex_step : PartialLex spec (wp ++ [head]) = some (seed_ts ++ [ExtChar.eos], []) := by
+            simp[PartialLex, PartialLex_seed] at h₀ ⊢
+            rw[h₀]
+            simp[PartialLex_trans, hh, hempty]
+            exact he
+
+          have lex_wr_step : (BuildLexingFST spec).eval [] = some (LexingState.start, []) := by
+            simp[BuildLexingFST, Id.run, FST.eval, FST.evalFrom]
+
+          have ih := ih (wp ++ [head]) LexingState.start (seed_ts ++ [ExtChar.eos]) [] hplex_step hlex_wp_step lex_wr_step
+
+          simp[hh] at hlex_trans
+          rw[hlex_trans]
+          simp at ih
+          convert ih
+          simp[hempty]
+        .  -- we have no transition and must show thats the case for both of them
+          simp[hempty]
+          -- since seed_wr ≠ [], q' is not start
+          have hq'_not_start : q' ≠ LexingState.start := by
+            exact (Iff.ne h₃).mp hempty
+          -- and so, the corresponding fsa state is the fst state
+          simp[LexingState.src] at h₂_fsa
+          cases hq' : q'
+          case neg.start => contradiction
+          rename_i src
+          -- in particular, its not accepting
+          have hlex_step : ((BuildLexingFST spec).evalFrom_fold_step (some (LexingState.id src, seed_ts)) ExtChar.eos) = none := by
+            simp[FST.evalFrom_fold_step, BuildLexingFST, Id.run]
+            simp[FSA.accepts_iff] at haccept ⊢
+            simp[hq', h₂_fsa] at haccept
+            simp[haccept]
+
+          simp[hq', haccept, h₂_fsa, hlex_step]
+    case char ch =>
+      cases hstep : spec.automaton.step (LexingState.src spec q') ch
+      case none =>
+        simp_all
+        by_cases haccept : LexingState.src spec q' ∈ spec.automaton.accept
+        case pos =>
+          let qsrc := LexingState.src spec q'
+          let term := spec.term qsrc
+          let unwrapped := term.get ((spec.hterm qsrc).mp haccept)
+          cases hch : spec.automaton.step spec.automaton.start ch
+          case none =>
+            -- no transition in both if ch is not in the prefix language
+            have : PartialLex_trans spec (some (seed_ts, seed_wr)) (ExtChar.char ch) = none := by
+              simp[PartialLex_trans]
+              simp[FSA.evalFrom_append]
+              simp[h₂_fsa, hh, hstep, haccept]
+              simp[FSA.evalFrom, hstep]
+              simp[hch]
+            simp[this]
+            have : ((BuildLexingFST spec).evalFrom_fold_step (some (q', seed_ts)) (ExtChar.char ch)) = none := by
+              simp[BuildLexingFST, Id.run, FST.evalFrom_fold_step]
+              simp[hh, hch, hstep, haccept]
+            simp[this]
+          case some qnext =>
+            have hplex_step : PartialLex_trans spec (some (seed_ts, seed_wr)) (ExtChar.char ch) = some (seed_ts ++ [ExtChar.char unwrapped], [ch]) := by
+              simp[PartialLex_trans, hh]
+              simp[FSA.evalFrom_append]
+              simp[h₂_fsa, hh, haccept]
+              simp[FSA.evalFrom, hstep]
+              simp[unwrapped, term, qsrc]
+              simp[hch]
+
+            have hplex_trans : PartialLex spec (wp ++ [head]) = some (seed_ts ++ [ExtChar.char unwrapped], [ch]) := by
+              simp[PartialLex_seed] at h₀ ⊢
+              rw[h₀]
+              simp[hh]
+              exact hplex_step
+
+            have hlex_wp_step : (BuildLexingFST spec).evalFrom_fold_step (some (q', seed_ts)) (ExtChar.char ch) = some (LexingState.id qnext, seed_ts ++ [ExtChar.char unwrapped]) := by
+              simp[FST.evalFrom_fold_step, BuildLexingFST, Id.run]
+              simp[h₂_fsa, hstep, haccept]
+              simp[hch, unwrapped, term, qsrc]
+
+            have hlex_wp_trans : (BuildLexingFST spec).eval (wp ++ [head]) = some (LexingState.id qnext, seed_ts ++ [ExtChar.char unwrapped]) := by
+              simp[FST.evalFrom, FST.eval] at h₁ ⊢
+              rw[←FST.evalFrom_fold_eq_evalFrom] at h₁ ⊢
+              simp[FST.evalFrom_fold, FST.evalFrom_fold_seed] at h₁ ⊢
+              rw[h₁]
+              simp[hh]
+              exact hlex_wp_step
+
+            have lex_wr_step : (BuildLexingFST spec).eval [ch] = some (LexingState.id qnext, []) := by
+              simp[BuildLexingFST, Id.run, FST.eval, FST.evalFrom]
+              simp[LexingState.src, hch]
+
+            have ih := ih (wp ++ [head]) (LexingState.id qnext) (seed_ts ++ [ExtChar.char unwrapped]) [ch] hplex_trans hlex_wp_trans lex_wr_step (by simp[hh])
+            rw[hplex_step]
+            rw[hlex_wp_step]
+            unfold FST.evalFrom_fold_seed at ih
+            exact ih
+        case neg =>
+          have : PartialLex_trans spec (some (seed_ts, seed_wr)) (ExtChar.char ch) = none := by
+            simp[PartialLex_trans, hh]
+            simp[FSA.evalFrom_append]
+            simp[h₂_fsa, FSA.evalFrom, hstep, haccept]
+          simp[this]
+          have : ((BuildLexingFST spec).evalFrom_fold_step (some (q', seed_ts)) (ExtChar.char ch)) = none := by
+            simp[BuildLexingFST, Id.run, FST.evalFrom_fold_step]
+            simp[hh, hstep, haccept]
+          simp[this]
+      case some dst =>
+        -- both will effectively take the transition specified by automata
+        have hplex_step : PartialLex_trans spec (some (seed_ts, seed_wr)) (ExtChar.char ch) = some (seed_ts, seed_wr ++ [ch]) := by
+          simp[PartialLex_trans, hh]
+          simp[FSA.evalFrom_append]
+          simp[h₂_fsa, hh]
+          simp[FSA.evalFrom, hstep]
+
+        have hplex_trans : PartialLex spec (wp ++ [head]) = some (seed_ts, seed_wr ++ [ch]) := by
+          simp[PartialLex_seed] at h₀ ⊢
+          rw[h₀]
+          simp[hh]
+          exact hplex_step
+
+        have hlex_wp_step : (BuildLexingFST spec).evalFrom_fold_step (some (q', seed_ts)) (ExtChar.char ch) = some (LexingState.id dst, seed_ts) := by
+          simp[FST.evalFrom_fold_step, BuildLexingFST, Id.run]
+          simp[h₂_fsa, hstep]
+
+        have hlex_wp_trans : (BuildLexingFST spec).eval (wp ++ [head]) = some (LexingState.id dst, seed_ts) := by
+          simp[FST.evalFrom, FST.eval] at h₁ ⊢
+          rw[←FST.evalFrom_fold_eq_evalFrom] at h₁ ⊢
+          simp[FST.evalFrom_fold, FST.evalFrom_fold_seed] at h₁ ⊢
+          rw[h₁]
+          simp[hh]
+          exact hlex_wp_step
+
+        have lex_wr_step : (BuildLexingFST spec).eval (seed_wr ++ [ch]) = some (LexingState.id dst, []) := by
+          simp[FST.evalFrom, FST.evalFrom_append]
+          rw[←FST.evalFrom_fold_eq_evalFrom]
+          simp[FST.evalFrom_fold]
+          rw[h₂]
+          simp[BuildLexingFST, Id.run, hstep]
+
+        have ih := ih (wp ++ [head]) (LexingState.id dst) seed_ts (seed_wr ++ [ch]) hplex_trans hlex_wp_trans lex_wr_step (by simp[hh])
+        rw[hplex_step]
+        rw[hlex_wp_step]
+        unfold FST.evalFrom_fold_seed at ih
+        simp at ih
+        exact ih
+
+theorem PartialLex_to_LexingFST (spec: LexerSpec α Γ σ) (he: [] ∉ spec.automaton.accepts) :
+  ∀ w, match PartialLex spec w with
+       | some (ts', wr) =>
+          ∃ q', (BuildLexingFST spec).eval w = some (q', ts') ∧ (BuildLexingFST spec).eval wr = some (q', [])
+       | none => (BuildLexingFST spec).eval w = none := by
+
+  let fst := BuildLexingFST spec
+  let new_q0 := fst.start
+
+  have := PartialLex_to_LexingFST_evalFold spec he
+  intro w
+  have := this [] w new_q0 [] []
+  have := this rfl
+  have := this (by simp[FST.eval, fst, new_q0]) (by simp[FST.eval, fst, new_q0]) (by simp[new_q0, fst])
+  simp[PartialLex, fst] at this ⊢
+  rw[FST.evalFrom_fold_seed_eq_evalFrom_seed] at this
+  simp[FST.evalFrom_seed] at this
+  split
+  <;> simp_all
+  rename_i t'' wr _ _ _
+  obtain ⟨q'', hq⟩ := this
+  exists q''
+  split at hq
+  simp_all
+  rename_i heq
+  constructor
+  simp[←hq.left]
+  exact heq
+  rw[FST.evalFrom_fold_seed_eq_evalFrom_seed] at hq
+  simp[FST.evalFrom_seed] at hq
+  split at hq
+  try split at this
+  rename_i heq
+  simp at hq
+  simp[hq] at heq
+  simp_all
+  split at this
+  <;> simp_all
+  assumption
+
+
+theorem PartialLexRel_to_LexingFST (spec: LexerSpec α Γ σ) (he: [] ∉ spec.automaton.accepts) (hpruned: spec.automaton.pruned) :
+  ∀ w terminals unlexed,
+    PartialLexRel spec w terminals unlexed →
+      ∃ q', (BuildLexingFST spec).eval w = some (q', terminals)
+          ∧ (BuildLexingFST spec).eval unlexed = some (q', []) := by
+  intro w terminals unlexed h
+  have hpl := (PartialLex_pruned_eq_PartialLexRel spec hpruned w terminals unlexed).mp h
+  have := PartialLex_to_LexingFST spec he w
+  simp only [hpl] at this
+  obtain ⟨q', heval_w, heval_unlexed⟩ := this
+  exists q'
+
+theorem LexingFST_to_PartialLexRel (spec: LexerSpec α Γ σ) (he: [] ∉ spec.automaton.accepts) (hpruned: spec.automaton.pruned) :
+  ∀ w q' terminals,
+    (BuildLexingFST spec).eval w = some (q', terminals) →
+    ∃ (unlexed: List α),
+      (BuildLexingFST spec).eval unlexed = some (q', []) ∧ PartialLexRel spec w terminals unlexed := by
+  intro w q' terminals h
+  cases hpl : PartialLex spec w
+  case none =>
+    have : (BuildLexingFST spec).eval w = none := by
+      have := PartialLex_to_LexingFST spec he w
+      simp only [hpl] at this
+      exact this
+    simp at this
+    simp[this] at h
+  case some ts_wr =>
+    have ⟨ ts', wr⟩ := ts_wr
+    have := PartialLex_to_LexingFST spec he w
+    simp only [hpl] at this
+    obtain ⟨q'', heval_w, heval_wr⟩ := this
+    have heq : q'' = q' ∧ ts' = terminals := by
+      simp at h heval_w
+      simp[heval_w] at h
+      exact h
+    exists wr
+    simp at heval_wr ⊢
+    constructor
+    simp[heq] at heval_wr
+    exact heval_wr
+    have hrel := (PartialLex_pruned_eq_PartialLexRel spec hpruned w ts' wr).mpr
+    simp only [hpl, heq] at hrel
+    simp[hrel]
+
 namespace Detokenizing
 
 universe x
@@ -514,5 +985,3 @@ theorem detokenizer_comp { σ0 } ( tokens : List (Token α V)) (f : FST α Γ σ
     simp_all[h, Option.map, Prod.snd]
     cases f.evalFrom f.start u.2 <;> simp_all
   | none => simp_all
-
-end Detokenizing
